proof/Simple/BaseTactics.v
@@ -1,0 +1,12 @@
+
+Require Export Omega.
+Require Export BaseLibTactics.
+
+(* Tactics ************************************************)
+Tactic Notation "break" constr(E) :=
+ let X := fresh "X" in remember (E) as X; destruct X.
+
+Tactic Notation "breaka" constr(E) :=
+ let X := fresh "X" in remember (E) as X; destruct X; auto.
+
+
